use upper camel case and rename file

Cslib/Languages/LambdaCalculus/LocallyNameless/Untyped/LcAt.lean
@@ -29,11 +29,11 @@ LcAt k M is satisfied when all bound indices of M are smaller than k.
 When k = 0, this is equivalent to LC, as shown in lcAt_iff_LC.
 -/
 @[simp, scoped grind =]
-def lcAt (k : ℕ) : Term Var → Prop
+def LcAt (k : ℕ) : Term Var → Prop
 | bvar i => i < k
 | fvar _ => True
-| app t₁ t₂ => lcAt k t₁ ∧ lcAt k t₂
-| abs t => lcAt (k + 1) t
+| app t₁ t₂ => LcAt k t₁ ∧ LcAt k t₂
+| abs t => LcAt (k + 1) t
 
 /-- depth counts the maximum number of the lambdas that are enclosing variables. -/
 @[simp, scoped grind =]
@@ -79,18 +79,18 @@ lemma depth_openRec_fvar_eq_depth (M : Term Var) (x : Var) (i : ℕ) :
 theorem depth_open_fvar_eq_depth (M : Term Var) (x : Var) :
   depth (M ^ fvar x) = depth M := depth_openRec_fvar_eq_depth M x 0
 
-/-- Opening for some free variable at i-th bound variable, increases the lcAt by 1. -/
+/-- Opening for some free variable at i-th bound variable, increases the LcAt by 1. -/
 @[simp, scoped grind .]
 theorem lcAt_openRec_fvar_iff_lcAt (M : Term Var) (x : Var) (i : ℕ) :
-    lcAt i (M⟦i ↝ fvar x⟧) ↔ lcAt (i+1) M := by
+    LcAt i (M⟦i ↝ fvar x⟧) ↔ LcAt (i+1) M := by
   induction M generalizing i <;> grind
 
-/-- Opening for some free variable is locally closed if and only if M is lcAt 1. -/
+/-- Opening for some free variable is locally closed if and only if M is LcAt 1. -/
 theorem lcAt_open_fvar_iff_lcAt (M : Term Var) (x : Var) :
-   lcAt 0 (M ^ (fvar x)) ↔ lcAt 1 M := lcAt_openRec_fvar_iff_lcAt M x 0
+   LcAt 0 (M ^ (fvar x)) ↔ LcAt 1 M := lcAt_openRec_fvar_iff_lcAt M x 0
 
-/-- M is lcAt 0 if and only if M is locallly closed. -/
-theorem lcAt_iff_LC (M : Term Var) [HasFresh Var] : lcAt 0 M ↔ M.LC := by
+/-- M is LcAt 0 if and only if M is locallly closed. -/
+theorem lcAt_iff_LC (M : Term Var) [HasFresh Var] : LcAt 0 M ↔ M.LC := by
 induction M using LambdaCalculus.LocallyNameless.Untyped.Term.ind_on_depth with
   | h_abs =>
     constructor
